src/Store_Semantics_alt.v
@@ -1,0 +1,868 @@
+Require Import Term StructTactics Event_system Term_system.
+
+Require Import Lia Coq.Program.Tactics.
+
+
+Inductive store_event: Ev -> Loc -> Prop :=
+| put_event: forall i x p q t, store_event (req i x p q t) x
+| put_event_spl: forall i xi yi p, store_event (splitp i xi yi p) xi
+| put_event_spr: forall i xi yi p, store_event (splitp i xi yi p) yi
+| get_event: forall i x p q, store_event (rpy i x p q) x
+| get_event_joinpl: forall i xi yi p, store_event (joinp i xi yi p) xi
+| get_event_joinpr: forall i xi yi p, store_event (joinp i xi yi p) yi.
+
+Lemma wf_mono_locs: forall t,
+    well_formed t ->
+    fst (lrange t) <= snd (lrange t).
+Proof.
+  intros.
+  rewrite Term.well_formed_lrange; eauto.
+  lia.
+Defined.
+
+Ltac inv_wf :=
+  match goal with
+  | [H: well_formed (aasp _ _ _) |- _] =>
+    invc H
+  | [H: well_formed (alseq _ _ _ _) |- _] =>
+    invc H
+  | [H: well_formed (aatt _ _ _ _ ?t) |- _] =>   
+    invc H
+  | [H: well_formed (abseq _ _ _ _ _) |- _] =>
+    invc H
+  | [H: well_formed (abpar _ _ _ _ _ _ _) |- _] =>
+    invc H
+  end.
+
+Ltac inv_ev :=
+  match goal with
+  | [H: events (aasp _ _ _) _ _ |- _] =>
+    invc H
+  | [H: events (alseq _ _ _ _) _ _ |- _] =>
+    invc H
+  | [H: events (aatt _ _ _ _ _) _ _ |- _] =>   
+    invc H
+  | [H: events (abseq _ _ _ _ _) _ _ |- _] =>
+    invc H
+  | [H: events (abpar _ _ _ _ _ _ _) _ _ |- _] =>
+    invc H
+  end.
+
+Ltac inv_ev' :=
+  match goal with
+  | [H: events (aasp _ _ _) _ _ |- _] =>
+    inv H
+  | [H: events (alseq _ _ _ _) _ _ |- _] =>
+    inv H
+  | [H: events (aatt _ _ _ _ _) _ _ |- _] =>   
+    inv H
+  | [H: events (abseq _ _ _ _ _) _ _ |- _] =>
+    inv H
+  | [H: events (abpar _ _ _ _ _ _ _) _ _ |- _] =>
+    inv H
+  end.
+
+Ltac inv_ev2 :=
+  match goal with
+  | [H: events _ _ _,
+     H': events _ _ _ |- _] =>
+    invc H; invc H'
+  end.
+
+Ltac inv_ev2' :=
+  match goal with
+  | [H: events _ _ _,
+     H': events _ _ _ |- _] =>
+    inv H; inv H'
+  end.
+
+Create HintDb lr.
+
+Lemma rpy_events_lrange (t:AnnoTerm) : forall p i p1 q loc,
+    well_formed t ->
+    events t p (rpy i loc p1 q) ->
+    fst (lrange t) <= loc < snd (lrange t).
+Proof.
+  intros.
+  generalizeEverythingElse t.
+  induction t; intros;
+      try (
+        cbn in *;
+        inv_wf;
+        inv_ev;
+        simpl in *; subst;
+        try lia;
+        repeat (find_eapply_hyp_hyp);
+        repeat find_eapply_lem_hyp wf_mono_locs;
+        lia).
+Defined.
+Hint Resolve rpy_events_lrange : lr.
+
+Lemma req_events_lrange (t:AnnoTerm) : forall p i p1 q t0 loc,
+    well_formed t ->
+    events t p (req i loc p1 q  t0) ->
+    fst (lrange t) <= loc < snd (lrange t).
+Proof.
+  intros.
+  generalizeEverythingElse t.
+  induction t; intros;
+    try (
+        cbn in *;
+        inv_wf;
+        inv_ev;
+        simpl in *; subst;
+        try lia;
+        repeat (find_eapply_hyp_hyp);
+        repeat find_eapply_lem_hyp wf_mono_locs;
+        lia).
+Defined.
+Hint Resolve req_events_lrange : lr.
+
+Lemma splitp_l_events_lrange (t:AnnoTerm) : forall p i p0 yi loc,
+    well_formed t ->
+    events t p (splitp i loc yi p0) ->
+    fst (lrange t) <= loc < snd (lrange t).
+Proof.
+  intros.
+  generalizeEverythingElse t.
+  induction t; intros;
+    try (
+        cbn in *;
+        inv_wf;
+        inv_ev;
+        simpl in *; subst;
+        try lia;
+        repeat (find_eapply_hyp_hyp);
+        repeat find_eapply_lem_hyp wf_mono_locs;
+        lia).
+Defined.
+Hint Resolve splitp_l_events_lrange : lr.
+
+Lemma splitp_r_events_lrange (t:AnnoTerm) : forall p i p0 xi loc,
+    well_formed t ->
+    events t p (splitp i xi loc p0) ->
+    fst (lrange t) <= loc < snd (lrange t).
+Proof.
+  intros.
+  generalizeEverythingElse t.
+  induction t; intros;
+    try (
+        cbn in *;
+        inv_wf;
+        inv_ev;
+        simpl in *; subst;
+        try lia;
+        repeat (find_eapply_hyp_hyp);
+        repeat find_eapply_lem_hyp wf_mono_locs;
+        lia).
+Defined.
+Hint Resolve splitp_r_events_lrange : lr.
+
+Lemma joinp_l_events_lrange (t:AnnoTerm) : forall p p0 i yi loc,
+    well_formed t ->
+    events t p (joinp i loc yi p0) ->
+    fst (lrange t) <= loc < snd (lrange t).
+Proof.
+  intros.
+  generalizeEverythingElse t.
+  induction t; intros;
+    try (
+        cbn in *;
+        inv_wf;
+        inv_ev;
+        simpl in *; subst;
+        try lia;
+        repeat (find_eapply_hyp_hyp);
+        repeat find_eapply_lem_hyp wf_mono_locs;
+        lia).
+Defined.
+Hint Resolve joinp_l_events_lrange : lr.
+
+Lemma joinp_r_events_lrange (t:AnnoTerm) : forall p p0 i xi loc,
+    well_formed t ->
+    events t p (joinp i xi loc p0) ->
+    fst (lrange t) <= loc < snd (lrange t).
+Proof.
+  intros.
+  generalizeEverythingElse t.
+  induction t; intros;
+    try (
+        cbn in *;
+        inv_wf;
+        inv_ev;
+        simpl in *; subst;
+        try lia;
+        repeat (find_eapply_hyp_hyp);
+        repeat find_eapply_lem_hyp wf_mono_locs;
+        lia).
+Defined.
+Hint Resolve joinp_r_events_lrange : lr.
+
+Lemma store_events_lrange (t:AnnoTerm) : forall p ev loc,
+    well_formed t ->
+    events t p ev ->
+    store_event ev loc ->
+    fst (lrange t) <= loc < snd (lrange t).
+Proof.
+  intros.
+  inv H1;
+    eauto with lr.
+Defined.
+
+Ltac pose_store_events :=
+  match goal with
+  | [H: events _ _ ?ev,
+        H': Loc |- _] =>
+    assert_new_proof_by (store_event ev H') econstructor
+  end.
+
+Ltac pose_new_lrange :=
+  match goal with
+  | [H: well_formed ?t,
+        H': events ?t ?p ?ev,
+            H'': store_event ?ev ?loc
+     |- _] =>
+    pose_new_proof (store_events_lrange t p ev loc H H' H'')
+  end.
+
+Ltac pose_lrange_facts :=
+  repeat pose_store_events;
+  repeat pose_new_lrange;
+  repeat find_eapply_lem_hyp wf_mono_locs.
+
+Ltac dest_lrange :=
+  match goal with
+  | [H: LocRange |- _] => destruct H
+  end.
+
+Create HintDb rl.
+
+Lemma unique_req_locs: forall t p i i0 loc p0 p1 q q0 t0 t1,
+    well_formed t ->
+    events t p (req i loc p0 q t0) ->
+    events t p (req i0 loc p1 q0 t1) ->
+    i = i0.
+Proof.
+  intros.
+  generalizeEverythingElse t.
+  induction t; intros;
+    inv_wf;
+    inv_ev2;
+    try eauto;
+    dest_lrange; simpl in *;
+      try (pose_lrange_facts;    
+           lia).
+Defined.
+Hint Resolve unique_req_locs : rl.
+
+Lemma unique_req_splitp_l_locs:
+  forall (t : AnnoTerm) (p i i0 loc p0 p1 q yi : nat) (t0: Term),
+    well_formed t ->
+    events t p (req i loc p0 q t0) ->
+    events t p (splitp i0 loc yi p1) -> i = i0.
+Proof.
+  intros.
+  generalizeEverythingElse t.
+  induction t; intros;
+    inv_wf;
+    inv_ev2;
+    try eauto;
+    dest_lrange; simpl in *;
+      try (pose_lrange_facts;    
+           lia).
+Defined.
+Hint Resolve unique_req_splitp_l_locs : rl.
+
+Lemma unique_req_splitp_r_locs:
+  forall (t : AnnoTerm) (p i i0 loc p0 p1 q xi : nat) (t0: Term),
+    well_formed t ->
+    events t p (req i loc p0 q t0) ->
+    events t p (splitp i0 xi loc p1) -> i = i0.
+Proof.
+  intros.
+  generalizeEverythingElse t.
+  induction t; intros;
+    inv_wf;
+    inv_ev2;
+    try eauto;
+    dest_lrange; simpl in *;
+      try (pose_lrange_facts;    
+           lia).
+Defined.
+Hint Resolve unique_req_splitp_r_locs: rl.
+
+Lemma unique_req_rpy_locs
+  : forall (t : AnnoTerm) (p i i0 loc p0 p1 q q0 : nat) (t0: Term),
+    well_formed t ->
+    events t p (req i loc p0 q t0) ->
+    events t p (rpy i0 loc p1 q0) -> i = i0.
+Proof.
+  intros.
+  generalizeEverythingElse t.
+  induction t; intros;
+    inv_wf;
+    inv_ev2;
+    try eauto;
+    dest_lrange; simpl in *;
+      try (pose_lrange_facts;    
+           lia).
+Defined.
+Hint Resolve unique_req_rpy_locs: rl.
+
+Lemma unique_splitp_splitp_ll_locs:
+  forall (t : AnnoTerm) (p i i0 loc p0 p1 yi yi0 : nat),
+    well_formed t ->
+    events t p (splitp i  loc yi  p0) ->
+    events t p (splitp i0 loc yi0 p1) -> i = i0.
+Proof.
+  intros.
+  generalizeEverythingElse t.
+  induction t; intros;
+    inv_wf;
+    inv_ev2;
+    try eauto;
+    dest_lrange; simpl in *;
+      try (pose_lrange_facts;    
+           lia).
+Defined.
+Hint Resolve unique_splitp_splitp_ll_locs: rl.
+
+Lemma unique_splitp_splitp_rl_locs:
+  forall (t : AnnoTerm) (p i i0 loc p0 p1 yi yi0 : nat),
+    well_formed t ->
+    events t p (splitp i0 loc yi0 p1) ->
+    events t p (splitp i  yi loc  p0) ->
+    i = i0.
+Proof.
+  intros.
+  generalizeEverythingElse t.
+  induction t; intros;
+    inv_wf;
+    inv_ev2;
+    try eauto;
+    dest_lrange; simpl in *;
+      try (pose_lrange_facts;    
+           lia).
+Defined.
+Hint Resolve unique_splitp_splitp_rl_locs: rl.
+
+Lemma unique_rpy_splitp_l_locs:
+  forall (t : AnnoTerm) (p i i0 loc p0 p1 q yi : nat),
+    well_formed t ->
+    events t p (rpy i loc p0 q) ->
+    events t p (splitp i0 loc yi p1) -> i = i0.
+Proof.
+  intros.
+  generalizeEverythingElse t.
+  induction t; intros;
+    inv_wf;
+    inv_ev2;
+    try eauto;
+    dest_lrange; simpl in *;
+      try (pose_lrange_facts;    
+           lia).
+Defined.
+Hint Resolve unique_rpy_splitp_l_locs: rl.
+
+Lemma unique_splitp_splitp_rr_locs:
+  forall (t : AnnoTerm) (p i i0 loc p0 p1 xi xi0 : nat),
+    well_formed t ->
+    events t p (splitp i  xi loc  p0) ->
+    events t p (splitp i0 xi0 loc p1) -> i = i0.
+Proof.
+  intros.
+  generalizeEverythingElse t.
+  induction t; intros;
+    inv_wf;
+    inv_ev2;
+    try eauto;
+    dest_lrange; simpl in *;
+      try (pose_lrange_facts;    
+           lia).
+Defined.
+Hint Resolve unique_splitp_splitp_rr_locs: rl.
+
+Lemma unique_rpy_splitp_r_locs:
+  forall (t : AnnoTerm) (p i i0 loc p0 p1 q xi : nat),
+    well_formed t ->
+    events t p (rpy i loc p0 q) ->
+    events t p (splitp i0 xi loc p1) -> i = i0.
+Proof.
+  intros.
+  generalizeEverythingElse t.
+  induction t; intros;
+    inv_wf;
+    inv_ev2;
+    try eauto;
+    dest_lrange; simpl in *;
+      try (pose_lrange_facts;    
+           lia).
+Defined.
+Hint Resolve unique_rpy_splitp_r_locs: rl.
+
+Lemma unique_rpy_locs
+  : forall (t : AnnoTerm) (p i i0 loc p0 p1 q q0 : nat),
+    well_formed t ->
+    events t p (rpy i  loc p0 q) ->
+    events t p (rpy i0 loc p1 q0) -> i = i0.
+Proof.
+  intros.
+  generalizeEverythingElse t.
+  induction t; intros;
+    inv_wf;
+    inv_ev2;
+    try eauto;
+    dest_lrange; simpl in *;
+      try (pose_lrange_facts;    
+           lia).
+Defined.
+Hint Resolve unique_rpy_locs: rl.
+
+Lemma unique_splitpl_joinpl_locs
+  : forall (t : AnnoTerm) (p i i0 loc p1 q0 yi yi' : nat),
+    well_formed t ->
+    events t p (splitp i loc yi p1) ->
+    events t p (joinp i0 loc yi' q0) ->
+    i = i0.
+Proof.
+  intros.
+  generalizeEverythingElse t.
+  induction t; intros;
+    inv_wf;
+    inv_ev2;
+    try eauto;
+    dest_lrange; simpl in *;
+      try (pose_lrange_facts;    
+           lia).
+Defined.
+Hint Resolve unique_splitpl_joinpl_locs: rl.
+
+Lemma unique_req_joinpl_locs
+  : forall (t : AnnoTerm) (p i i0 loc p0 q q0 yi : nat) t0,
+    well_formed t ->
+    events t p (req i loc p0 q t0) ->
+    events t p (joinp i0 loc yi q0) ->
+    i = i0.
+Proof.
+  intros.
+  generalizeEverythingElse t.
+  induction t; intros;
+    inv_wf;
+    inv_ev2;
+    try eauto;
+    dest_lrange; simpl in *;
+      try (pose_lrange_facts;    
+           lia).
+Defined.
+Hint Resolve unique_req_joinpl_locs: rl.
+
+Lemma unique_splitpr_joinpl_locs
+  : forall (t : AnnoTerm) (p i i0 loc p1 q0 xi yi : nat),
+    well_formed t ->
+    events t p (splitp i xi loc p1) ->
+    events t p (joinp i0 loc yi q0) ->
+    i = i0.
+Proof.
+  intros.
+  generalizeEverythingElse t.
+  induction t; intros;
+    inv_wf;
+    inv_ev2;
+    try eauto;
+    dest_lrange; simpl in *;
+      try (pose_lrange_facts;    
+           lia).
+Defined.
+Hint Resolve unique_splitpr_joinpl_locs: rl.
+
+Lemma unique_rpy_joinpl_locs
+  : forall (t : AnnoTerm) (p i i0 loc p0 q q0 yi : nat),
+    well_formed t ->
+    events t p (rpy i loc p0 q) ->
+    events t p (joinp i0 loc yi q0) ->
+    i = i0.
+Proof.
+  intros.
+  generalizeEverythingElse t.
+  induction t; intros;
+    inv_wf;
+    inv_ev2;
+    try eauto;
+    dest_lrange; simpl in *;
+      try (pose_lrange_facts;    
+           lia).
+Defined.
+Hint Resolve unique_rpy_joinpl_locs: rl.
+
+Lemma unique_joinpl_joinpl_locs
+  : forall (t : AnnoTerm) (p i i0 loc p1 q0 yi yi' : nat),
+    well_formed t ->
+    events t p (joinp i  loc yi p1) ->
+    events t p (joinp i0 loc yi' q0) ->
+    i = i0.
+Proof.
+  intros.
+  generalizeEverythingElse t.
+  induction t; intros;
+    inv_wf;
+    inv_ev2;
+    try eauto;
+    dest_lrange; simpl in *;
+      try (pose_lrange_facts;    
+           lia).
+Defined.
+Hint Resolve unique_joinpl_joinpl_locs: rl.
+
+Lemma unique_req_joinpr_locs
+  : forall (t : AnnoTerm) (p i i0 loc p0 q q0 xi : nat) t0,
+    well_formed t ->
+    events t p (req i loc p0 q t0) ->
+    events t p (joinp i0 xi loc q0) ->
+    i = i0.
+Proof.
+  intros.
+  generalizeEverythingElse t.
+  induction t; intros;
+    inv_wf;
+    inv_ev2;
+    try eauto;
+    dest_lrange; simpl in *;
+      try (pose_lrange_facts;    
+           lia).
+Defined.
+Hint Resolve unique_req_joinpr_locs: rl.
+
+Lemma unique_splitpl_joinpr_locs
+  : forall (t : AnnoTerm) (p i i0 loc p1 q0 yi xi : nat),
+    well_formed t ->
+    events t p (splitp i loc yi p1) ->
+    events t p (joinp i0 xi loc q0) ->
+    i = i0.
+Proof.
+  intros.
+  generalizeEverythingElse t.
+  induction t; intros;
+    inv_wf;
+    inv_ev2;
+    try eauto;
+    dest_lrange; simpl in *;
+      try (pose_lrange_facts;    
+           lia).
+Defined.
+Hint Resolve unique_splitpl_joinpr_locs: rl.
+
+Lemma unique_splitpr_joinpr_locs
+  : forall (t : AnnoTerm) (p i i0 loc p1 q0 xi xi' : nat),
+    well_formed t ->
+    events t p (splitp i xi loc p1) ->
+    events t p (joinp i0 xi' loc q0) ->
+    i = i0.
+Proof.
+  intros.
+  generalizeEverythingElse t.
+  induction t; intros;
+    inv_wf;
+    inv_ev2;
+    try eauto;
+    dest_lrange; simpl in *;
+      try (pose_lrange_facts;    
+           lia).
+Defined.
+Hint Resolve unique_splitpr_joinpr_locs: rl.
+
+Lemma unique_rpy_joinpr_locs
+  : forall (t : AnnoTerm) (p i i0 loc p0 q q0 xi : nat),
+    well_formed t ->
+    events t p (rpy i loc p0 q) ->
+    events t p (joinp i0 xi loc q0) ->
+    i = i0.
+Proof.
+  intros.
+  generalizeEverythingElse t.
+  induction t; intros;
+    inv_wf;
+    inv_ev2;
+    try eauto;
+    dest_lrange; simpl in *;
+      try (pose_lrange_facts;    
+           lia).
+Defined.
+Hint Resolve unique_rpy_joinpr_locs: rl.
+
+Lemma unique_joinpl_joinpr_locs
+  : forall (t : AnnoTerm) (p i i0 loc p1 q0 xi yi : nat),
+    well_formed t ->
+    events t p (joinp i  xi loc p1) ->
+    events t p (joinp i0 loc yi q0) ->
+    i = i0.
+Proof.
+  intros.
+  generalizeEverythingElse t.
+  induction t; intros;
+    inv_wf;
+    inv_ev2;
+    try eauto;
+    dest_lrange; simpl in *;
+      try (pose_lrange_facts;    
+           lia).
+Defined.
+Hint Resolve unique_joinpl_joinpr_locs: rl.
+
+Lemma unique_joinpr_joinpr_locs
+  : forall (t : AnnoTerm) (p i i0 loc p1 q0 xi xi' : nat),
+    well_formed t ->
+    events t p (joinp i  xi  loc p1) ->
+    events t p (joinp i0 xi' loc q0) ->
+    i = i0.
+Proof.
+  intros.
+  generalizeEverythingElse t.
+  induction t; intros;
+    inv_wf;
+    inv_ev2;
+    try eauto;
+    dest_lrange; simpl in *;
+      try (pose_lrange_facts;    
+           lia).
+Defined.
+Hint Resolve unique_joinpr_joinpr_locs: rl.
+
+
+Ltac flip a :=
+  try (eapply a;
+       eauto; tauto);
+  try (symmetry;
+       eapply a;
+       eauto; tauto);
+  tauto.
+
+Ltac dorl' a b c d e f g h i j k l m n o p q r s t u :=
+    first
+      [ flip a
+      | flip b
+      | flip c
+      | flip d
+      | flip e
+      | flip f
+      | flip g
+      | flip h
+      | flip i
+      | flip j
+      | flip k
+      | flip l
+      | flip m
+      | flip n
+      | flip o
+      | flip p
+      | flip q
+      | flip r
+      | flip s
+      | flip t
+      | flip u
+      ].
+
+Ltac dorl :=
+  dorl'
+    unique_req_locs
+    unique_req_splitp_l_locs
+    unique_req_splitp_r_locs
+    unique_req_rpy_locs
+    unique_req_joinpl_locs
+    unique_splitp_splitp_ll_locs
+    unique_splitp_splitp_rl_locs
+    unique_rpy_splitp_l_locs
+    unique_splitpl_joinpl_locs
+    unique_splitp_splitp_rr_locs
+    unique_rpy_splitp_r_locs
+    unique_splitpr_joinpl_locs
+    unique_rpy_locs
+    unique_rpy_joinpl_locs
+    unique_joinpl_joinpl_locs
+    unique_req_joinpr_locs
+    unique_splitpl_joinpr_locs
+    unique_splitpr_joinpr_locs
+    unique_rpy_joinpr_locs
+    unique_joinpl_joinpr_locs
+    unique_joinpr_joinpr_locs.
+    
+Lemma unique_store_events: forall t p ev1 ev2 loc,
+  well_formed t ->
+  events t p ev1 ->
+  events t p ev2 ->
+  store_event ev1 loc ->
+  store_event ev2 loc ->
+  ev1 = ev2.
+Proof.
+  intros.
+  eapply events_injective; eauto.
+  invc H2;
+    invc H3;
+    simpl;
+    try dorl.
+Defined.
+
+Lemma unique_store_events': forall t p ev1 ev2 loc,
+    well_formed t ->
+    ev_in ev1 (ev_sys t p) ->
+    ev_in ev2 (ev_sys t p) -> 
+    store_event ev1 loc ->
+    store_event ev2 loc ->
+    ev1 <> ev2 ->
+    False.
+Proof.
+  intros.
+  assert (ev1 = ev2).
+  {
+    eapply unique_store_events;
+      try eassumption.
+    eapply evsys_events; eauto.
+    eapply evsys_events; eauto.
+  }
+  congruence.
+Defined.
+
+Definition store_event_evsys es loc := exists ev, store_event ev loc /\ ev_in ev es.
+
+Inductive store_conflict: EvSys Ev -> Prop :=
+| store_conflict_merge: forall r es1 es2 loc,
+    store_event_evsys es1 loc ->
+    store_event_evsys es2 loc ->
+    store_conflict (merge r es1 es2)
+| store_conflict_before_l: forall r es1 es2,
+    store_conflict es1 ->
+    store_conflict (before r es1 es2)
+| store_conflict_before_r: forall r es1 es2,
+    store_conflict es2 ->
+    store_conflict (before r es1 es2).
+
+Lemma unique_events': forall r es1 es2 ev1 ev2,
+    well_structured ev (merge r es1 es2) ->
+    ev_in ev1 es1 ->
+    ev_in ev2 es2 ->
+    ev ev1 <> ev ev2.
+Proof.
+  intros.
+  inv H.
+  assert (fst (es_range es1) <= ev ev1 < snd (es_range es1)).
+  {
+    eapply ws_evsys_range; eauto.
+  }
+
+  assert (fst (es_range es2) <= ev ev2 < snd (es_range es2)).
+  {
+    eapply ws_evsys_range; eauto.
+  }
+
+  lia.
+Defined.
+
+Lemma unqev: forall ev1 ev2,
+  ev ev1 <> ev ev2 ->
+  ev1 <> ev2.
+Proof.
+  intros.
+  unfold not; intros.
+  subst.
+  solve_by_inversion.
+Defined.
+
+Lemma unique_events: forall r es1 es2 ev1 ev2,
+    well_structured ev (merge r es1 es2) ->
+    ev_in ev1 es1 ->
+    ev_in ev2 es2 ->
+    ev1 <> ev2.
+Proof.
+  intros.
+  eapply unqev.
+  eapply unique_events';
+    eauto.
+Defined.
+
+Theorem no_store_conflicts: forall t p sys,
+    well_formed t ->
+    sys = ev_sys t p ->
+    not (store_conflict sys).
+Proof.
+  unfold not; intros.
+  generalizeEverythingElse t.
+  induction t; intros.
+  -
+    destruct a;
+      cbn in *;
+      repeat break_let;
+      subst;
+      solve_by_inversion.
+  -
+    cbn in *;
+      repeat break_let;
+      subst.
+    inv H1.
+    +
+      solve_by_inversion.
+    +
+      inv H2;
+        try solve_by_inversion;
+        try inv_wf; eauto.
+      
+  -
+    cbn in *;
+      repeat break_let;
+      subst.
+    inv H1;
+      do_wf_pieces.
+  -
+    cbn in *;
+      repeat break_let;
+      subst.
+    inv H1.
+    +
+      solve_by_inversion.
+    +
+      inv H2.
+      ++
+        inv H3;
+          do_wf_pieces.
+      ++
+        solve_by_inversion.
+  -
+    
+    assert (well_structured ev sys).
+    {
+      rewrite H0.
+      eapply well_structured_evsys.
+      eassumption.
+    }
+    
+    cbn in *;
+      repeat break_let;
+      subst.
+    inv H1;
+      try solve_by_inversion.
+    +
+      inv H3;
+        try solve_by_inversion.
+      ++       
+        inv H4;
+          try solve_by_inversion.
+        +++
+          unfold store_event_evsys in *.
+          destruct_conjs.
+
+          assert (ev_in H6 (merge (S n, Nat.pred n0) (ev_sys t1 p1) (ev_sys t2 p1))).
+          {
+            eauto.
+          }
+          
+          assert (ev_in H8 (merge (S n, Nat.pred n0) (ev_sys t1 p1) (ev_sys t2 p1))).
+          {
+            eauto.
+          }
+
+          eapply unique_store_events' with (ev1:=H6) (ev2:=H8) (t:=(abpar (n, n0) l (n1,n2) (n3,n4) s t1 t2)) (p:=p1) (loc:=loc);
+            try eassumption;
+            try (simpl; eauto; tauto).
+          ++++  
+            inv H2.
+            inv H16.
+            eapply unique_events; eauto.
+Defined.
